Add InstructionNotFomalized
This is a preparation for skipping tests that involve precompiled contracts.

Hoare/Hoare.thy
@@ -342,7 +342,13 @@ definition instruction_result_as_set :: "constant_ctx \<Rightarrow> instruction_
           InstructionContinue v \<Rightarrow> {ContinuingElm True} \<union> contexts_as_set v c
         | InstructionToEnvironment act v _ \<Rightarrow> {ContinuingElm False, ContractActionElm act} \<union> contexts_as_set v c
         | InstructionAnnotationFailure \<Rightarrow> {ContinuingElm False} (* need to assume no annotation failure somewhere *)
+        | InstructionNotYetFormalized \<Rightarrow> {}
         )"
+
+lemma not_formalized_as_set [simp] :
+  "instruction_result_as_set co_ctx InstructionNotYetFormalized = {}"
+apply (simp add: instruction_result_as_set_def)
+done
 
 lemma annotation_failure_as_set [simp] :
   "instruction_result_as_set c InstructionAnnotationFailure = {ContinuingElm False}"
@@ -965,5 +971,7 @@ declare sep_sep_code [simp]
 (* validity of pre, program, post triples.
  * Failures are considered as success.
  *)
+
+
 
 end
